src/Std/Data/DTreeMap/Internal/WF/Lemmas.lean
@@ -1632,6 +1632,75 @@ theorem WF.eraseMany! {_ : Ord α} [TransOrd α] {ρ} [ForIn Id ρ α] {l : ρ}
     {t : Impl α β} (h : t.WF) : (t.eraseMany! l).1.WF :=
   (t.eraseMany! l).2 h (fun _ _ h' => h'.erase!)
 
+theorem eraseManyEntries!_eq_foldl {_ : Ord α} {l : List ((a : α) × β a)} {t : Impl α β} :
+    (t.eraseManyEntries! l).val = l.foldl (init := t) fun acc ⟨k, _⟩ => acc.erase! k := by
+  simp [eraseManyEntries!, ← List.foldl_hom Subtype.val, List.forIn_pure_yield_eq_foldl]
+
+theorem eraseManyEntries_eq_foldl {_ : Ord α} {l : List ((a : α) × β a)} {t : Impl α β} (h : t.Balanced) :
+    (t.eraseManyEntries l h).val = l.foldl (init := t) fun acc ⟨k, _⟩ => acc.erase! k := by
+  simp [eraseManyEntries, erase_eq_erase!, ← List.foldl_hom Subtype.val, List.forIn_pure_yield_eq_foldl]
+
+theorem eraseManyEntries_eq_foldl_impl {_ : Ord α} {t₁ : Impl α β} (h₁ : t₁.Balanced) {t₂ : Impl α β} :
+    (t₁.eraseManyEntries t₂ h₁).val = t₂.foldl (init := t₁) fun acc k _ => acc.erase! k := by
+  simp [foldl_eq_foldl]
+  rw [← eraseManyEntries_eq_foldl]
+  rotate_left
+  · exact h₁
+  · simp only [eraseManyEntries, pure, ForIn.forIn, Id.run_bind]
+    rw [forIn_eq_forIn_toListModel]
+    congr
+
+theorem eraseManyEntries!_eq_foldl_impl {_ : Ord α} {t₁ : Impl α β} {t₂ : Impl α β} :
+    (t₁.eraseManyEntries! t₂).val = t₂.foldl (init := t₁) fun acc k _ => acc.erase! k := by
+  simp [foldl_eq_foldl]
+  rw [← eraseManyEntries!_eq_foldl]
+  simp only [eraseManyEntries!, pure, ForIn.forIn, Id.run_bind]
+  rw [forIn_eq_forIn_toListModel]
+  congr
+
+theorem eraseManyEntries_eq_eraseManyEntries!_impl {_ : Ord α}
+    {t₁ t₂ : Impl α β} (h : t₁.Balanced) :
+    (t₁.eraseManyEntries t₂ h).val = (t₁.eraseManyEntries! t₂).val := by
+  simp only [eraseManyEntries_eq_foldl_impl, eraseManyEntries!_eq_foldl_impl]
+
+theorem eraseManyEntries_impl_perm_eraseList {_ : Ord α} [BEq α] [LawfulBEqOrd α] [TransOrd α]
+    {t₁ : Impl α β} (h₁ : t₁.WF) {t₂ : Impl α β} :
+    List.Perm (t₁.eraseManyEntries t₂ h₁.balanced).val.toListModel (t₁.toListModel.eraseList t₂.toListModel) := by
+  rw [eraseManyEntries_eq_foldl_impl]
+  rw [foldl_eq_foldl]
+  induction t₂.toListModel generalizing t₁ with
+  | nil => rfl
+  | cons e es ih =>
+    simp only [eraseList, List.foldl_cons]
+    apply List.Perm.trans (@ih (t₁.erase! e.1) (h₁.erase!))
+    apply eraseList_perm_of_perm_first
+    · apply toListModel_erase!
+      · exact h₁.balanced
+      · exact h₁.ordered
+    · apply h₁.erase!.ordered.distinctKeys
+
+theorem toListModel_eraseManyEntries_impl {_ : Ord α} [BEq α] [LawfulBEqOrd α] [TransOrd α]
+    {t₁ : Impl α β} (h₁ : t₁.WF) {t₂ : Impl α β} :
+    List.Perm (t₁.eraseManyEntries t₂ h₁.balanced).val.toListModel (t₁.toListModel.filter (fun p => !containsKey p.fst t₂.toListModel)) := by
+  apply List.Perm.trans
+  · apply eraseManyEntries_impl_perm_eraseList h₁
+  · apply eraseList_perm_filter_containsKey
+    · exact h₁.ordered.distinctKeys
+
+theorem toListModel_eraseManyEntries!_impl {_ : Ord α} [BEq α] [LawfulBEqOrd α] [TransOrd α]
+    {t₁ : Impl α β} (h₁ : t₁.WF) {t₂ : Impl α β} :
+    List.Perm (t₁.eraseManyEntries! t₂).val.toListModel (t₁.toListModel.filter (fun p => !containsKey p.fst t₂.toListModel)) := by
+  rw [← eraseManyEntries_eq_eraseManyEntries!_impl h₁.balanced]
+  apply toListModel_eraseManyEntries_impl h₁
+
+/-!
+### `eraseMany!`
+-/
+
+theorem WF.eraseManyEntries! {_ : Ord α} [TransOrd α] {ρ} [ForIn Id ρ ((a : α) × β a)] {l : ρ}
+    {t : Impl α β} (h : t.WF) : (t.eraseManyEntries! l).1.WF :=
+  (t.eraseManyEntries! l).2 h (fun _ _ h' => h'.erase!)
+
 /-!
 ### `insertMany`
 -/
